series + parallel extensions

Matroid/Extension.lean
@@ -3,44 +3,17 @@ import Matroid.Closure
 import Matroid.Minor.Basic
 import Matroid.Constructions.ImagePreimage
 import Matroid.ForMathlib.Other
-open Set
+
+open Set Function
 namespace Matroid
 
 variable {M : Matroid α}
 
+section Set
+
 /-- Replace the elements of `S` with parallel copies of `e`. -/
-def ParallelExt (M : Matroid α) (e : α) (S : Set α) [DecidablePred (· ∈ S)] : Matroid α :=
+def parallelExtendSet (M : Matroid α) (e : α) (S : Set α) [DecidablePred (· ∈ S)] : Matroid α :=
     M.preimage (fun x ↦ if (x ∈ S) then e else x)
-
-theorem insert_diff_insert_diff {B : Set α} (e_in_B : e ∈ B) (f_notin_B : f ∉ B):
-    insert e (insert f (B \ {e}) \ {f}) = B := by simp [e_in_B, f_notin_B]
-
-theorem Equiv.image_invol [DecidableEq α] {e f : α} :
-    Function.Involutive (Set.image (Equiv.swap e f)) := by
-  have inv : Function.Involutive (Equiv.swap e f) := fun x ↦ Equiv.swap_apply_self _ _ _
-  intro X
-  rw [←Set.image_comp _ _, Function.Involutive.comp_self inv, image_id]
-
-theorem Equiv.swap_image_eq_self [DecidableEq α] {S : Set α} (hef : e ∈ S ↔ f ∈ S) :
-    (Equiv.swap e f) '' S = S := by
-  ext x
-  rw [image_equiv_eq_preimage_symm, mem_preimage, Equiv.symm_swap, Equiv.swap_apply_def]
-  split_ifs with hxe hxf
-  · rwa [hxe, Iff.comm]
-  · rwa [hxf]
-  rfl
-
-theorem Equiv.swap_image_eq_exchange [DecidableEq α] {S : Set α} (he : e ∈ S) (hf : f ∉ S) :
-    (Equiv.swap e f) '' S = insert f (S \ {e}) := by
-  ext x
-  rw [image_equiv_eq_preimage_symm, mem_preimage, Equiv.symm_swap, Equiv.swap_apply_def,
-    mem_insert_iff, mem_diff]
-  split_ifs with hxe hxf
-  · subst hxe
-    simp [he, hf, (show x ≠ f by rintro rfl; exact hf he)]
-  · subst hxf
-    simp [he]
-  simp [hxe, iff_false_intro hxf]
 
 /-- Swapping two parallel elements gives an automorphism -/
 def parallel_swap [DecidableEq α] {M : Matroid α} {e f : α} (h_para : M.Parallel e f) : Iso M M :=
@@ -63,131 +36,264 @@ def parallel_swap [DecidableEq α] {M : Matroid α} {e f : α} (h_para : M.Paral
 @[simp] theorem parallel_swap_apply [DecidableEq α] (h_para : M.Parallel e f) :
     (parallel_swap h_para).toLocalEquiv = (Equiv.swap e f).toLocalEquiv.restr M.E := rfl
 
-theorem filter_preimage_eq {e f : α} [DecidableEq α] {S : Set α} (he : e ∈ S) (hf : f ∈ S)
-    (h_ne : e ≠ f) : (fun x ↦ if (x = e) then f else x) ⁻¹' (S \ {e}) = S := by
-  ext x
-  simp only [preimage_diff, mem_diff, mem_preimage, mem_singleton_iff]
-  split_ifs with hxe
-  · subst hxe
-    exact iff_of_true ⟨hf, h_ne.symm⟩ he
-  rw [and_iff_left hxe]
-
-open Classical
-theorem eq_parallelExt_del {M : Matroid α} {e f : α} (h_para : M.Parallel e f) (h_ne : e ≠ f):
-    M = ParallelExt (M ⟍ f) e {f} := by
-  rw [ParallelExt, eq_iff_indep_iff_indep_forall, preimage_ground_eq]
+end Set
 
 
-  refine' ⟨_, fun I I_ground ↦ ⟨fun I_Ind ↦ _, _⟩⟩
-  · simp only [mem_singleton_iff, delete_elem, delete_ground]
-    rw [filter_preimage_eq (h_para.mem_ground_right) (h_para.mem_ground_left) h_ne.symm]
-  · rw [preimage_indep_iff]
-    simp only [delete_elem, mem_singleton_iff, delete_indep_iff, disjoint_singleton_right,
-      mem_image, not_exists, not_and, delete_ground, union_singleton, mem_diff, not_true, and_false,
-      insert_diff_singleton]
-    constructor
-    · constructor
-      · by_cases f_in_I : f ∈ I
-        · have image_eq : (fun a ↦ if a = f then e else a) '' I = insert e (I \ {f})
-          · apply subset_antisymm
-            · rintro i ⟨a, a_I, h_a₁⟩
-              dsimp at h_a₁
-              by_cases a_eq_f : a = f
-              · rw [if_pos a_eq_f] at h_a₁
-                rw [←h_a₁]
-                exact mem_insert _ _
-              · rw [if_neg a_eq_f] at h_a₁
-                rw [←h_a₁]
-                exact mem_insert_of_mem _ (mem_diff_singleton.2 ⟨a_I, a_eq_f⟩)
-            · rintro i (i_eq_e | ⟨i_in_I, (i_ne_f : i ≠ f)⟩)
-              · refine' ⟨f, f_in_I, _⟩
-                rw [i_eq_e]
-                exact if_pos rfl
-              · refine ⟨i, i_in_I, if_neg i_ne_f⟩
-          rw [image_eq]
-          apply I_Ind.parallel_substitute h_para.symm f_in_I
-        · have image_eq : (fun a ↦ if a = f then e else a) '' I = I
-          · apply subset_antisymm
-            · rintro i ⟨a, a_I, h_a₁⟩
-              dsimp at h_a₁
-              rw [if_neg (ne_of_mem_of_not_mem a_I f_in_I)] at h_a₁
-              rwa [←h_a₁]
-            · rintro i i_in_I
-              refine' ⟨i, i_in_I, if_neg (ne_of_mem_of_not_mem i_in_I f_in_I)⟩
-          rwa [image_eq]
-      · intro x _
-        by_cases x_eq_f : x = f
-        · rwa [if_pos x_eq_f]
-        · rwa [if_neg x_eq_f]
+section Loop
 
-    --refine' ⟨_, subset_trans I_ground (subset_insert f M.E)⟩
-    rintro a a_I b b_I f_ab
-    dsimp at f_ab
-    by_cases b_eq_f : b = f
-    · rw [if_pos b_eq_f, ite_eq_left_iff] at f_ab
-      by_cases a_eq_f : a = f
-      · rwa [b_eq_f]
-      · have ef_sub_I : {e, f} ⊆ I
-        · rintro i (i_eq_e | (i_eq_f : i = f))
-          · rwa [i_eq_e, ←(f_ab a_eq_f)]
-          · rwa [i_eq_f, ←b_eq_f]
-        exfalso
-        apply I_Ind.not_dep _
-        rw [dep_iff_superset_circuit]
-        exact ⟨{e, f}, ef_sub_I, (parallel_iff_circuit h_ne).1 h_para⟩
-    · rw [if_neg b_eq_f] at f_ab
-      by_cases a_eq_f : a = f
-      · rw [if_pos a_eq_f] at f_ab
-        have ef_sub_I : {e, f} ⊆ I
-        · rintro i (i_eq_e | (i_eq_f : i = f))
-          · rwa [i_eq_e, f_ab]
-          · rwa [i_eq_f, ←a_eq_f]
-        exfalso
-        apply I_Ind.not_dep _
-        rw [dep_iff_superset_circuit]
-        exact ⟨{e, f}, ef_sub_I, (parallel_iff_circuit h_ne).1 h_para⟩
-      · rwa [if_neg a_eq_f] at f_ab
-  -- part 2
-  rw [preimage_indep_iff]
+variable {α : Type*} {M M' : Matroid α} {e : α}
 
-  rintro ⟨(I_image_Indep : (M ⟍ f).Indep ((fun x ↦ if x = f then e else x) '' I)), h_inj⟩
-  by_cases f_in_I : f ∈ I
-  · have image_eq : (fun a ↦ if a = f then e else a) '' I = insert e (I \ {f})
-    · apply subset_antisymm
-      · rintro i ⟨a, a_I, h_a₁⟩
-        dsimp at h_a₁
-        by_cases a_eq_f : a = f
-        · rw [if_pos a_eq_f] at h_a₁
-          rw [←h_a₁]
-          exact mem_insert _ _
-        · rw [if_neg a_eq_f] at h_a₁
-          rw [←h_a₁]
-          exact mem_insert_of_mem _ (mem_diff_singleton.2 ⟨a_I, a_eq_f⟩)
-      · rintro i (i_eq_e | ⟨i_in_I, (i_ne_f : i ≠ f)⟩)
-        · refine' ⟨f, f_in_I, _⟩
-          rw [i_eq_e]
-          exact if_pos rfl
-        · refine ⟨i, i_in_I, if_neg i_ne_f⟩
-    rw [image_eq] at I_image_Indep
-    have:= I_image_Indep.of_delete.parallel_substitute h_para (mem_insert e _)
-    have e_notin_I : e ∉ I
-    · intro e_in_I
-      apply h_ne (h_inj e_in_I f_in_I _)
-      dsimp
-      simp
-    rwa [←insert_diff_insert_diff f_in_I e_notin_I]
-  · have image_eq : (fun a ↦ if a = f then e else a) '' I = I
-    · apply subset_antisymm
-      · rintro i ⟨a, a_I, h_a₁⟩
-        dsimp at h_a₁
-        rw [if_neg (ne_of_mem_of_not_mem a_I f_in_I)] at h_a₁
-        rwa [←h_a₁]
-      · intro i i_in_I
-        refine' ⟨i, i_in_I, _⟩
-        exact if_neg (ne_of_mem_of_not_mem i_in_I f_in_I)
-    rw [image_eq] at I_image_Indep
-    exact I_image_Indep.of_delete
---another definition of "modularity" exists in the repo- is such that a base is modular over a set
---subsets if for any subset of that set, the intersection of the base with the intersection of
---that subset is a base for the intersection of the subset - cant find what exactly this means wrt
---modular pairs
+/-- Add a loop `e` to a matroid `M`. Has the junk value `M` if `e ∈ M.E` -/
+def addLoop (M : Matroid α) (e : α) : Matroid α := M ↾ (insert e M.E)
+
+theorem addLoop_eq_self (he : e ∈ M.E) : M.addLoop e = M := by
+  rw [addLoop, insert_eq_of_mem he, restrict_ground_eq_self]
+
+@[simp] theorem addLoop_ground (M : Matroid α) (e : α) : (M.addLoop e).E = insert e M.E := rfl
+
+@[simp] theorem addLoop_indep_iff : (M.addLoop f).Indep I ↔ M.Indep I := by
+  simp only [addLoop, restrict_indep_iff, and_iff_left_iff_imp]
+  exact fun hI ↦ hI.subset_ground.trans (subset_insert _ _)
+
+theorem eq_addLoop_iff (he : e ∉ M.E) : M' = M.addLoop e ↔ M'.Loop e ∧ M' ⟍ e = M := by
+  obtain (he' | he') := em' (e ∈ M'.E)
+  · refine iff_of_false ?_ ?_
+    · rintro rfl; simp at he'
+    rintro ⟨h, rfl⟩; exact he' h.mem_ground
+
+  simp_rw [delete_elem, eq_iff_indep_iff_indep_forall, addLoop_ground, addLoop_indep_iff,
+    delete_ground, delete_indep_iff, disjoint_singleton_right, ← singleton_dep, dep_iff,
+    singleton_subset_iff, and_iff_left he', subset_diff, disjoint_singleton_right, and_imp]
+
+  refine ⟨fun ⟨hE, hi⟩ ↦ ⟨?_, ?_, ?_⟩, fun ⟨hi, hE, h⟩ ↦ ⟨?_, fun I hIss ↦ ?_⟩⟩
+  · rw [hi _ (singleton_subset_iff.2 he')]
+    exact fun hei ↦ he (singleton_subset_iff.1 hei.subset_ground)
+  · simp [hE, he]
+  · rintro I hIss heI
+    rw [and_iff_left heI, hi _ hIss]
+  · rw [← hE, insert_diff_singleton, insert_eq_of_mem he']
+  obtain (heI | heI) := em (e ∈ I)
+  · exact iff_of_false (fun hI ↦ hi <| hI.subset (singleton_subset_iff.2 heI))
+      (fun hI ↦ he <| hI.subset_ground heI)
+  specialize h I hIss
+  simpa [heI] using h
+
+theorem addLoop_loop (he : e ∉ M.E) : (M.addLoop e).Loop e := by
+  rw [addLoop, ← singleton_dep, Dep, singleton_subset_iff, restrict_indep_iff,
+    singleton_subset_iff, restrict_ground_eq, and_iff_left (mem_insert _ _),
+    and_iff_left (mem_insert _ _)]
+  exact fun hi ↦ he (singleton_subset_iff.1 hi.subset_ground)
+
+def addColoop (M : Matroid α) (e : α) : Matroid α := (M﹡.addLoop e)﹡
+
+theorem addColoop_eq_self (he : e ∈ M.E) : M.addColoop e = M := by
+  rwa [addColoop, addLoop_eq_self, dual_dual]
+
+@[simp] theorem addColoop_ground (M : Matroid α) (e : α) : (M.addColoop e).E = insert e M.E := rfl
+
+theorem eq_addColoop_iff (he : e ∉ M.E) : M' = M.addColoop e ↔ M'.Coloop e ∧ M' ⟋ e = M := by
+  rw [addColoop, eq_dual_comm, eq_comm, eq_addLoop_iff (show e ∉ M﹡.E from he),
+    dual_loop_iff_coloop, eq_dual_comm, delete_elem, dual_delete_dual_eq_contract, contract_elem,
+    eq_comm]
+
+end Loop
+
+section Parallel
+
+variable {α : Type*} [DecidableEq α] {M : Matroid α}
+
+/-- Replace `f` with a parallel copy of `e` in `M`. Intended for use where `e` is a nonloop
+  and `f ∉ M.E`. When this is not the case, the junk value is described by
+  either `parallelExtend_not_nonloop` or `parallelExtend_delete_mem_eq` -/
+def parallelExtend (M : Matroid α) (e f : α) : Matroid α :=
+  (M.preimage (update id f e)) ↾ (insert f M.E)
+
+@[simp] theorem parallelExtend_ground (M : Matroid α) (e f : α) :
+    (M.parallelExtend e f).E = insert f M.E := rfl
+
+@[simp] theorem parallelExtend_self (M : Matroid α) (e : α) :
+    M.parallelExtend e e = M.addLoop e := by
+  change preimage _ (update id e (id e)) ↾ _ = _
+  rw [update_eq_self, preimage_id, addLoop]
+
+theorem parallelExtend_not_nonloop (he : ¬M.Nonloop e) (f : α) :
+    M.parallelExtend e f = (M ⟍ f).addLoop f := by
+  classical
+  simp only [parallelExtend, delete_elem, eq_iff_indep_iff_indep_forall, restrict_ground_eq,
+    addLoop_ground, delete_ground, mem_diff, mem_singleton_iff, not_true_eq_false, and_false,
+    insert_diff_singleton, restrict_indep_iff, preimage_indep_iff, ne_eq, image_update, id_eq,
+    image_id', update_id_injOn_iff, addLoop_indep_iff, delete_indep_iff, disjoint_singleton_right,
+    true_and]
+  rintro I hI
+  split_ifs with hf
+  · simp [(show ¬ M.Indep (insert e _) from fun hi ↦ he <| hi.nonloop_of_mem (mem_insert _ _)), hf]
+  simp [hf, hI]
+
+theorem parallelExtend_eq_parallelExtend_delete (M : Matroid α) {e f : α} (hef : e ≠ f):
+    M.parallelExtend e f = (M ⟍ f).parallelExtend e f := by
+  classical
+  rw [parallelExtend, parallelExtend, delete_elem, delete_ground, insert_diff_singleton,
+    eq_iff_indep_iff_indep_forall]
+  simp only [restrict_ground_eq, restrict_indep_iff, preimage_indep_iff, ne_eq, image_update, id_eq,
+    image_id', mem_diff, mem_singleton_iff, update_id_injOn_iff, delete_indep_iff,
+    disjoint_singleton_right, and_congr_left_iff, iff_self_and, true_and]
+  aesop
+
+theorem parallelExtend_delete_eq' (M : Matroid α) (e f : α) :
+    (M.parallelExtend e f) ⟍ f = M ⟍ f := by
+  classical
+  simp only [parallelExtend, delete_elem, eq_iff_indep_iff_indep_forall, delete_ground,
+    restrict_ground_eq, mem_insert_iff, true_or, not_true_eq_false, mem_singleton_iff,
+    insert_diff_of_mem, subset_diff, disjoint_singleton_right, delete_indep_iff, restrict_indep_iff,
+    preimage_indep_iff, ne_eq, image_update, id_eq, image_id', mem_diff, update_id_injOn_iff,
+    and_congr_left_iff, and_imp, true_and]
+  rintro I - hf -
+  simp only [hf, not_false_eq_true, diff_singleton_eq_self, ite_false, IsEmpty.forall_iff, and_true,
+    and_iff_left_iff_imp]
+  exact fun hI ↦ hI.subset_ground.trans <| subset_insert _ _
+
+theorem parallelExtend_delete_eq (e : α) (hf : f ∉ M.E) : (M.parallelExtend e f) ⟍ f = M := by
+  rwa [parallelExtend_delete_eq', delete_elem, delete_eq_self_iff, disjoint_singleton_left]
+
+theorem parallelExtend_nonloop_iff (he : M.Nonloop e) :
+    (M.parallelExtend e f).Nonloop x ↔ M.Nonloop x ∨ x = f := by
+  classical
+  rw [← indep_singleton, parallelExtend, restrict_indep_iff, singleton_subset_iff,
+    preimage_indep_iff, and_iff_left (injOn_singleton _ _), mem_insert_iff,
+    image_update, image_id, image_id]
+
+  obtain (rfl | hne) := eq_or_ne x f
+  · simpa
+  simp only [mem_singleton_iff, hne.symm, not_false_eq_true, diff_singleton_eq_self, ite_false,
+    indep_singleton, hne, false_or, or_false, and_iff_left_iff_imp]
+  exact Nonloop.mem_ground
+
+theorem parallelExtend_parallel (he : M.Nonloop e) (f : α) :
+    (M.parallelExtend e f).Parallel e f := by
+  classical
+  have he' : (M.parallelExtend e f).Nonloop e
+  · rw [parallelExtend_nonloop_iff he]; left; assumption
+  have hf : (M.parallelExtend e f).Nonloop f
+  · rw [parallelExtend_nonloop_iff he]; right; rfl
+  obtain (rfl | hef) := eq_or_ne e f
+  · rwa [parallel_self_iff]
+  rw [he'.parallel_iff_dep hf hef, Dep, pair_subset_iff, and_iff_right he'.mem_ground,
+    and_iff_left hf.mem_ground, parallelExtend, restrict_indep_iff, preimage_indep_iff,
+    image_update, image_id, image_id,
+    if_pos (mem_insert_of_mem _ (show f ∈ ({f} : Set α) from rfl))]
+  exact fun hcon ↦ hef <| hcon.1.2 (by simp) (by simp) (by simp [update_noteq hef e id])
+
+theorem parallelExtend_indep_iff (he : M.Nonloop e) (hf : f ∉ M.E) :
+    (M.parallelExtend e f).Indep I ↔
+      (f ∉ I ∧ M.Indep I) ∨ (f ∈ I ∧ e ∉ I ∧ M.Indep (insert e (I \ {f}))) := by
+  have hdel : ∀ J, f ∉ J → ((M.parallelExtend e f).Indep J ↔ M.Indep J)
+  · rintro J hfJ
+    convert (delete_indep_iff (M := M.parallelExtend e f) (D := {f}) (I := J)).symm using 1
+    · rw [disjoint_singleton_right, and_iff_left hfJ]
+    rw [← delete_elem, parallelExtend_delete_eq', delete_elem, delete_indep_iff,
+      disjoint_singleton_right, and_iff_left hfJ]
+  have hef : e ≠ f
+  · rintro rfl; exact hf he.mem_ground
+
+  obtain (hfI | hfI) := em (f ∈ I)
+  · rw [iff_true_intro hfI, not_true, false_and, false_or, true_and]
+    obtain (heI | heI) := em (e ∈ I)
+    · simp only [heI, not_true_eq_false, mem_diff, mem_singleton_iff, true_and, false_and,
+        iff_false, parallelExtend_ground]
+      exact fun hi ↦ ((parallelExtend_parallel he f).dep_of_ne hef).not_indep
+        (hi.subset (pair_subset heI hfI))
+    rw [and_iff_right heI, (parallelExtend_parallel he f).symm.indep_substitute_iff hfI heI, hdel]
+    rintro (rfl | h); exact hef rfl
+    exact h.2 rfl
+
+  simp [hdel _ hfI, hfI]
+
+theorem eq_parallelExtend_iff (he : M.Nonloop e) (hf : f ∉ M.E) :
+    M' = M.parallelExtend e f ↔ M'.Parallel e f ∧ M' ⟍ f = M := by
+  have hef : e ≠ f := by rintro rfl; exact hf he.mem_ground
+  constructor
+  · rintro rfl
+    exact ⟨parallelExtend_parallel he f, parallelExtend_delete_eq _ hf⟩
+  rintro ⟨hpar, rfl⟩
+  apply eq_of_indep_iff_indep_forall
+  · simp [insert_eq_of_mem hpar.mem_ground_right]
+  rintro I -
+  simp_rw [parallelExtend_indep_iff he hf, delete_elem, delete_indep_iff]
+  simp only [disjoint_singleton_right, mem_diff, mem_singleton_iff, mem_insert_iff,
+    not_true_eq_false, and_false, or_false, and_iff_left hef.symm]
+  obtain (hfI | hfI) := em (f ∈ I)
+  · simp only [hfI, not_true_eq_false, and_false, and_self, mem_diff, mem_singleton_iff, true_and,
+      false_or]
+    obtain (heI | heI) := em (e ∈ I)
+    · simp only [heI, not_true_eq_false, mem_diff, mem_singleton_iff, true_and, false_and,
+        iff_false]
+      exact fun hI ↦ (hpar.dep_of_ne hef).not_indep (hI.subset <| pair_subset heI hfI)
+    rw [hpar.symm.indep_substitute_iff hfI heI, and_iff_right heI]
+  simp [hfI]
+
+end Parallel
+
+section Series
+
+variable {α : Type*} [DecidableEq α] {M : Matroid α}
+
+/-- Coextend `e` by `f` in series. Intended for use where `e` is a non-coloop
+  and `f ∉ M.E`. When this is not the case, the junk value is described by
+  either `seriesExtend_not_nonloop` or `seriesExtend_delete_mem_eq` -/
+def seriesExtend (M : Matroid α) (e f : α) : Matroid α := (M﹡.parallelExtend e f)﹡
+
+@[simp] theorem seriesExtend_dual (M : Matroid α) (e f : α) :
+    (M.seriesExtend e f)﹡ = M﹡.parallelExtend e f := by
+  rw [seriesExtend, dual_dual]
+
+@[simp] theorem parallelExtend_dual (M : Matroid α) (e f : α) :
+    (M.parallelExtend e f)﹡ = M﹡.seriesExtend e f := by
+  rw [seriesExtend, dual_dual]
+
+@[simp] theorem seriesExtend_ground (M : Matroid α) (e f : α) :
+    (M.seriesExtend e f).E = insert f M.E := rfl
+
+@[simp] theorem seriesExtend_self (M : Matroid α) (e : α) :
+    M.seriesExtend e e = M.addColoop e := by
+  rw [seriesExtend, parallelExtend_self, addColoop]
+
+theorem seriesExtend_coloop (he : M.Coloop e) (f : α) :
+    M.seriesExtend e f = (M ⟋ f).addColoop f := by
+  rw [seriesExtend, parallelExtend_not_nonloop, addColoop, contract_elem,
+    delete_elem, contract_dual_eq_dual_delete]
+  simp [Nonloop, dual_loop_iff_coloop, he]
+
+theorem seriesExtend_not_mem_ground (he : e ∉ M.E) (f : α) :
+    M.seriesExtend e f = (M ⟋ f).addColoop f := by
+  rw [seriesExtend, parallelExtend_not_nonloop, addColoop, contract_elem, delete_elem,
+    contract_dual_eq_dual_delete]
+  simp [Nonloop, he]
+
+theorem seriesExtend_eq_seriesExtend_contract (M : Matroid α) {e f : α} (hef : e ≠ f):
+    M.seriesExtend e f = (M ⟋ f).seriesExtend e f := by
+  rw [seriesExtend, parallelExtend_eq_parallelExtend_delete _ hef, seriesExtend]
+  simp only [delete_elem, contract_elem, contract_dual_eq_dual_delete]
+
+theorem seriesExtend_contract_eq' (M : Matroid α) (e f : α) :
+    (M.seriesExtend e f) ⟋ f = M ⟋ f := by
+  rw [seriesExtend, contract_elem, ← delete_dual_eq_dual_contract, ← delete_elem,
+    parallelExtend_delete_eq']
+  simp
+
+theorem seriesExtend_contract_eq (e : α) (hf : f ∉ M.E) : (M.seriesExtend e f) ⟋ f = M := by
+  rw [seriesExtend, contract_elem, ← delete_dual_eq_dual_contract, ← delete_elem,
+    parallelExtend_delete_eq _ (show f ∉ M﹡.E from hf), dual_dual]
+
+theorem seriesExtend_series (heE : e ∈ M.E) (he : ¬M.Coloop e) (f : α) :
+    (M.seriesExtend e f).Series e f := by
+  rw [Series, seriesExtend, dual_dual]
+  apply parallelExtend_parallel
+  rwa [Nonloop, dual_ground, and_iff_left heE, dual_loop_iff_coloop]
+
+theorem eq_seriesExtend_iff (heE : e ∈ M.E) (he : ¬M.Coloop e) (hf : f ∉ M.E) :
+    M' = M.seriesExtend e f ↔ M'.Series e f ∧ M' ⟋ f = M := by
+  rw [seriesExtend, eq_dual_comm, eq_comm, eq_parallelExtend_iff _ (show f ∉ M﹡.E from hf),
+    delete_elem, ← contract_dual_eq_dual_delete, ← contract_elem, dual_inj_iff, Series]
+  rwa [Nonloop, and_iff_left (show e ∈ M﹡.E from heE), dual_loop_iff_coloop]
+
+end Series
